coq syntax update for union calulus with intersection types

double_anno_inter/coq/typing_wvalue.v
@@ -2,13 +2,26 @@ Require Import TLC.LibLN.
 Require Import syntax_wvalue.
 
 (*
+This file is created on March 06, 2021
 
-Update start on April 04, 2021.
+This is the main semantics file for disjoint union types
+with intersection types.
 
-This is typing file for syntax_wvalue.
+syntax.v is the syntax file for this semantics
+
+This file contains type safety and deterministic lemmas
+associated with syntax_wvalue.v
+
+Bool and String primitive type
+
+Removed top from ordinary types
+
+April 06, 2021:
+--------------
+-> extended from typing_no_top_findsubtypes.v
+-> wexpr added
 
 *)
-
 
 (* defns dropanno *)
 Inductive dropanno : exp -> exp -> Prop :=    (* defn findtype *)
@@ -19,11 +32,18 @@ Inductive dropanno : exp -> exp -> Prop :=    (* defn findtype *)
      lc_exp (e_abs e) ->
      dropanno (e_abs e) (e_abs e).
 
+
 (* defns Typing *)
 Inductive typing : env -> exp -> dirflag -> typ -> Prop :=    (* defn typing *)
  | typ_lit : forall (G:env) i5,
       okt  G  ->
      typing G (e_lit i5) infer t_int
+ | typ_bool : forall (G:env) b,
+      okt  G  ->
+     typing G (e_bool b) infer t_bool
+ | typ_str : forall (G:env) s,
+      okt G ->
+      typing G (e_str s) infer t_str
  | typ_var : forall (G:env) (x:var) (A:typ),
       okt  G  ->
       binds  x A G  ->
@@ -54,6 +74,10 @@ Reserved Notation "e --> e'" (at level 80).
 Inductive step : exp -> exp -> Prop :=    (* defn step *)
  | step_int : forall i5,
      step (e_lit i5) (e_ann (e_lit i5) t_int)
+ | step_bool : forall b,
+     step (e_bool b) (e_ann (e_bool b) t_bool)
+ | step_str : forall s,
+     step (e_str s) (e_ann (e_str s) t_str)
  | step_appl : forall (e1 e2 e1':exp),
      lc_exp e2 ->
      step e1 e1' ->
@@ -62,19 +86,13 @@ Inductive step : exp -> exp -> Prop :=    (* defn step *)
      wexpr v ->
      step e e' ->
      step (e_app v e) (e_app v e')
- | step_beta : forall (e:exp) (A1 B1 A2 B2:typ) (v v1:exp),
+ | step_beta : forall (e:exp) (A1 B1 A2 B2:typ) (v v1:exp) (C:typ),
      lc_exp (e_abs e) ->
      value v ->
      dropanno v v1 ->
-     (e_app  ( (e_ann (e_ann  ( (e_abs e) )  (t_arrow A1 B1)) (t_arrow A2 B2)) ) (v) ) --> (e_ann (e_ann  (  (open_exp_wrt_exp  e (e_ann (e_ann v1 A2) A1) )  )  B1) B2)
-(*
-     | step_beta_abs : forall (e:exp) (A1 B1 A2 B2:typ) (p:exp) (C:typ) x,
-     lc_exp (e_abs e) ->
-     p = (e_abs x) ->
-     (e_app  ( (e_ann (e_ann  ( (e_abs e) )  (t_arrow A1 B1)) (t_arrow A2 B2)) ) ( p ) ) --> (e_ann (e_ann  (  (open_exp_wrt_exp  e (e_ann (e_ann p A2) A1) )  )  B1) B2)
-*)
-     | step_ann : forall (e:exp) (A:typ) (e':exp),
-      not ( wexpr (e_ann e A) )  ->
+     (e_app  ( (e_ann (e_ann  ( (e_abs e) )  (t_arrow A1 B1)) (t_arrow A2 B2)) ) ( v ) ) --> (e_ann (e_ann  (  (open_exp_wrt_exp  e (e_ann (e_ann v1 A2) A1) )  )  B1) B2)
+ | step_ann : forall (e:exp) (A:typ) (e':exp),
+     not ( wexpr (e_ann e A) )  ->
      step e e' ->
      step (e_ann e A) (e_ann e' A)
  | step_rm_ann : forall (p:exp) (A B:typ),
@@ -101,7 +119,6 @@ Inductive step : exp -> exp -> Prop :=    (* defn step *)
      step (e_typeof (e_ann p D) A e1 B e2)  (open_exp_wrt_exp  e2 (e_ann p B) )
 where "e --> e'" := (step e e') : env_scope.
 
-(** infrastructure *)
 Hint Constructors dropanno typing step : core.
 
 (** Gathering free names already used in the proofs *)
@@ -330,6 +347,8 @@ Lemma typing_weakening : forall E F G e dir T,
 Proof.
   introv Typ. gen F. inductions Typ; introv Ok.
   - apply* typ_lit.
+  - apply* typ_bool.
+  - apply* typ_str.
   - apply* typ_var. apply* binds_weaken.
   - apply* typ_ann.
   - apply* typ_app.
@@ -356,6 +375,8 @@ introv TypT TypU.
 lets TypT': TypT.
 inductions TypT; introv; simpl.
  - apply* typ_lit.
+ - apply* typ_bool.
+ - apply* typ_str.
  - case_var.
   + binds_get H0.
     lets M: (typing_weakening E F empty u infer U).
@@ -416,7 +437,8 @@ Lemma check_or_typ : forall E e A B,
 Proof.
   intros.
   inductions H1; try solve [ inverts* H | inverts* H0 | inverts* H1].
-  inverts* H. inverts* H1. inverts* H2. inverts* H1. inverts* H2.
+  inverts H;
+  inverts* H1; inverts* H2.
 Qed.
 
 Lemma check_pexpr_ann : forall E p A C,
@@ -428,6 +450,14 @@ intros E p A C Prev Typ.
 inductions Prev.
 - inverts Typ. inverts H. inverts H3. inverts H.
   assert (typing E (e_lit i5) infer t_int). eauto.
+  eapply typ_sub; eauto.
+  eapply sub_transitivity; eauto.
+- inverts Typ. inverts H. inverts H3. inverts H.
+  assert (typing E (e_bool b) infer t_bool). eauto.
+  eapply typ_sub; eauto.
+  eapply sub_transitivity; eauto.
+- inverts Typ. inverts H. inverts H3. inverts H.
+  assert (typing E (e_str s) infer t_str). eauto.
   eapply typ_sub; eauto.
   eapply sub_transitivity; eauto.
 - inverts Typ. inverts H0. inverts H4. inverts H0.
@@ -458,6 +488,12 @@ inductions Prev.
 - exists t_int. constructor. constructor.
   apply typing_regular in Typ. destruct~ Typ.
   dependent destruction Typ. dependent destruction Typ. auto.
+- exists t_bool. constructor. constructor.
+  apply typing_regular in Typ. destruct~ Typ.
+  dependent destruction Typ. dependent destruction Typ. auto.
+- exists t_str. constructor. constructor.
+  apply typing_regular in Typ. destruct~ Typ.
+  dependent destruction Typ. dependent destruction Typ. auto.
 - dependent destruction Typ.
   dependent destruction Typ.
   exists (t_arrow A0 B). constructor. auto. auto.
@@ -483,13 +519,13 @@ Proof.
   - (* app *)
     inverts* Red.
     + (* beta *)
-      inverts H4.
-     * inverts Typ1. 
+     inverts H4.
+     * inverts Typ1.
       do 3 dependent destruction H6.
       { (* infer lam *)
         dependent destruction H6.
       }
-      {
+      {  
         dependent destruction H3.
         constructor.
         pick_fresh x.
@@ -502,7 +538,7 @@ Proof.
         rewrite* concat_empty_r.
         rewrite H6.
       (* prove p:A1 checks *)
-        inverts* Typ2. inverts* H.
+        inverts Typ2. inverts H.
         assert (typing G (e_ann (e_ann v1 A) A1) infer A1).
         assert (B0 <: A1).
         eapply sub_transitivity; eauto.
@@ -528,6 +564,7 @@ Proof.
       assert (typing G ((e_ann (e_ann (e_abs e0) (t_arrow A2 B2)) A1)) infer A1). eauto.
       forwards*: typing_through_subst_ee.
       rewrite* (@subst_ee_intro y).
+      inverts H4.
   - (* typeof *)
     inverts* Red.
     + pick_fresh y. assert (y \notin L) by auto.
@@ -539,6 +576,14 @@ Proof.
       rewrite H7.
       dependent destruction H12.
       * assert (typing G (e_lit i5) infer t_int). apply typ_lit.
+        forwards*: typing_regular Typ.
+        forwards*: typing_through_subst_ee.
+        rewrite* (@subst_ee_intro y).
+      * assert (typing G (e_bool b) infer t_bool). apply typ_bool.
+        forwards*: typing_regular Typ.
+        forwards*: typing_through_subst_ee.
+        rewrite* (@subst_ee_intro y).
+      * assert (typing G (e_str s) infer t_str). apply typ_str.
         forwards*: typing_regular Typ.
         forwards*: typing_through_subst_ee.
         rewrite* (@subst_ee_intro y).
@@ -559,6 +604,14 @@ Proof.
         forwards*: typing_regular Typ.
         forwards*: typing_through_subst_ee.
         rewrite* (@subst_ee_intro y).
+      * assert (typing G (e_bool b) infer t_bool). apply typ_bool.
+        forwards*: typing_regular Typ.
+        forwards*: typing_through_subst_ee.
+        rewrite* (@subst_ee_intro y).
+      * assert (typing G (e_str s) infer t_str). apply typ_str.
+        forwards*: typing_regular Typ.
+        forwards*: typing_through_subst_ee.
+        rewrite* (@subst_ee_intro y).
       * assert (typing G (e_ann (e_abs e) (t_arrow A0 B0)) infer (t_arrow A0 B0)). apply typ_ann.
         do 4 dependent destruction Typ. auto.
         forwards*: typing_through_subst_ee.
@@ -576,9 +629,12 @@ Proof.
   clear st. gen_eq E: (@empty typ).  gen U1 U2.
   induction Typ; introv EQT EQE;
    try solve [ inverts* Val | inversion EQT | eauto ].
-    subst. assert (B <: (t_arrow U1 U2)). {
+  - inverts EQT. inverts H0.
+  - inverts EQT. inverts H0.
+  - inverts EQT. inverts H0.
+  - subst. assert (B <: (t_arrow U1 U2)). {
     eapply sub_transitivity. apply H. apply EQT. }
-   eapply IHTyp. apply Val. apply H0. reflexivity.
+    eapply IHTyp. apply Val. apply H0. auto.
 Qed.
 
 Lemma check_both_disj_false : forall E e A B,
@@ -588,15 +644,20 @@ Lemma check_both_disj_false : forall E e A B,
 Proof.
   intros.
   inductions H; try solve [ inverts* H | inverts* H0 | inverts* H2].
-  inverts H1. inverts H. inverts H2. inverts H.
-  unfold DisjSpec in H0. specialize (H0 t_int).
-  forwards*: H0. inverts H.
-  inverts H1. inverts H3. inverts H2. inverts H1.
-  unfold DisjSpec in H0.
-  specialize (H0 (t_arrow A0 B0)).
-  forwards*: H0. inverts H1.
+ - inverts H1. inverts H. inverts H2. inverts H.
+   unfold DisjSpec in H0. specialize (H0 t_int).
+   forwards*: H0.
+ - inverts H1. inverts H. inverts H2. inverts H.
+   unfold DisjSpec in H0. specialize (H0 t_bool).
+   forwards*: H0.
+ - inverts H1. inverts H. inverts H2. inverts H.
+   unfold DisjSpec in H0. specialize (H0 t_str).
+   forwards*: H0.
+ - inverts H1. inverts H3. inverts H2. inverts H1.
+   unfold DisjSpec in H0.
+   specialize (H0 (t_arrow A0 B0)).
+   forwards*: H0.
 Qed.
-
 
 Lemma not_expr : forall e t, ~ value (e_ann e t) -> ~ pexpr e.
 Proof.
@@ -610,20 +671,24 @@ Proof.
 introv lc. intros.
 inductions e; try solve [right; unfold not; intros; inversion H0].
 - left*.
+- left*.
+- left*.
 - inductions e; try solve [right; unfold not; intros; inverts H0].
   destruct~ IHe0. inversion lc. subst. auto. unfold not. intros. inversion H0.
   inductions t; try solve [ right; unfold not; intros; inversion H1].
   left. apply pexpr_abs. inversion lc; subst. auto.
 Qed.
 
-
 Lemma value_not_value : forall e, lc_exp e -> (wexpr e) \/ (~ (wexpr e)).
 Proof.
 introv lc.
+intros.
 inductions e;
-try solve [right; unfold not; intros; inversion H; inverts lc].
+try solve [right; unfold not; intros; inversion H].
 destruct~ IHe. inverts* lc.
 - inverts* H. inverts* H0.
+ + right. unfold not. intros. inversion H. subst. inversion H1.
+ + right. unfold not. intros. inversion H. subst. inversion H1.
  + right. unfold not. intros. inversion H. subst. inversion H1.
  + right. unfold not. intros. inverts H0. inversion H2.
 - apply val_pexpr in H.
@@ -639,16 +704,24 @@ introv Typ. gen_eq E: (@empty typ). lets Typ': Typ.
 inductions Typ; intros EQ; subst.
 (*case int*)
  - right*.
+ (*case bool*)
+ - right*.
+ (*case string*)
+ - right*.
+ (*case var*)
  - apply binds_empty_inv in H0. inversion H0.
+ (*case anno*)
  - destruct* IHTyp.
   + inverts H.
-    * inverts H0.
-      right. exists (e_ann p A). apply* step_rm_ann.
-    * inverts Typ. inverts H.
-      right. exists (e_ann (e_ann (e_abs e0)(t_arrow A0 B))(t_arrow A0 B) ).
-      apply* step_lam_ann.
+  (*case step-rm-anno*)
+   * inverts H0.
+     right. exists (e_ann p A). apply* step_rm_ann.
+   (*case step-lam-ann*)
+   * inverts Typ. inverts H.
+     right. exists (e_ann (e_ann (e_abs e0)(t_arrow A0 B))(t_arrow A0 B) ).
+     apply* step_lam_ann.
   + destruct H.
-     dependent destruction Typ. 
+    dependent destruction Typ.
      { inverts* Typ.
        { apply binds_empty_inv in H2. inversion H2. }
        { 
@@ -660,7 +733,7 @@ inductions Typ; intros EQ; subst.
          destruct (value_not_value ((e_ann (e_ann (e_ann p A0) B) A))).
          forwards*: typing_regular Typ'.
          left*.
-         right. exists*.
+         right.  exists*.
        }
        { right. exists (e_ann x A). apply* step_ann.
          unfold not. intros. inversion H3. inversion H5. 
@@ -672,23 +745,32 @@ inductions Typ; intros EQ; subst.
  - right. destruct* IHTyp1.
   + destruct* IHTyp2.
    * inverts* H.
-    inverts* H1. inverts Typ1. inverts H. 
-    inverts H3. inverts H. inverts H1.
+    inverts* H1. inverts Typ1. inverts H.
+    (*i infers arrow*)
+    inverts H3. inverts H. inverts H1. inverts H.
+    (*b infers arrow*)
+    inverts H3. inverts H. inverts H1. inverts H.
+    (*s infers arrow*)
+    inverts H3. inverts H. inverts H1. inverts H.
+    (*beta-reduction*)
     inverts H0. inverts H.
     exists* (e_ann (e_ann (open_exp_wrt_exp e (e_ann (e_ann p A) A0)) B0) B).
     exists* (e_ann (e_ann (open_exp_wrt_exp e (e_ann (e_ann (e_abs e0) A) A0)) B0) B).
     inverts Typ1.
+    (*case step-appr*)
    * destruct H0.
-   destruct H.
+     destruct H.
    { exists* (e_app e x). }
-   { inverts Typ1. } 
-  + destruct H.
+   { inverts Typ1. }
+   (*case step-appl*)
+  + destruct H. 
     exists (e_app x e2). apply* step_appl.
     forwards*: typing_regular Typ2.
+ (*case typ-sub*)
  - destruct~ IHTyp.
- - left. forwards*:typing_regular Typ'.
-   destruct~ H1. inverts* H2. 
- - right. destruct* IHTyp. 
+ - left. forwards*: typing_regular Typ'.
+   destruct~ H1. inverts* H2.
+ - right. destruct* IHTyp.
   + inverts H4. inverts H5. 
     apply check_pexpr_ann in Typ; auto.
     eapply check_or_typ in Typ; eauto.
@@ -701,7 +783,8 @@ inductions Typ; intros EQ; subst.
      lets: H y H6.
      eapply step_typeofl with (C:=S); eauto.
      forwards*: typing_regular Typ'.
-     inverts H5; inverts* H41. inversion H4.
+     inverts H5; inverts* H41.
+     inversion H4. 
      inverts H4. eauto. inversion H4.
    * forwards*: pexpr_inf_typ H4.
      destruct H6 as [S [H41 H51]].
@@ -715,7 +798,7 @@ inductions Typ; intros EQ; subst.
      inversion H4.
      inverts H4. eauto.
      inversion H4.
-   * inverts Typ. inverts H4.  
+   * inverts Typ. inversion H4.
   + destruct H4.
      exists (e_typeof x A e1 B e2).
      apply step_typeof; auto.
@@ -727,239 +810,172 @@ e --> e1 -> e --> e2 -> e1 = e2.
 Proof.
   introv Typ He1. gen e2 A dir.
   induction He1; introv Typ He2.
-(*case step-int*)
+  (*case step-int*)
   - inverts* He2.
-(*case step-appl*)
+  (*case step-bool*)
+  - inverts* He2.
+  (*case step-str*) 
+  - inverts* He2.
+  (*case step-appl*)
   - inverts* He2.
    + inverts Typ.
      forwards*: IHHe1. rewrite* H0.
      inverts H0. eapply typ_sub with (A:=(t_arrow A0 B)) in H7; eauto.
      forwards*: IHHe1. rewrite* H0.
    + inverts* H2. inverts* H0. 
-    * inverts* He1.
-      assert (value (e_ann (e_lit i5) A0)). eauto.
+    * inverts He1. assert (value (e_ann (e_lit i5) A0)) by auto. 
       inverts H0. contradiction.
-    * inverts* He1.
+    * inverts He1. assert (value (e_ann (e_bool b) A0)) by auto. 
+      inverts H0. contradiction.
+    * inverts He1. assert (value (e_ann (e_str s) A0)) by auto. 
+      inverts H0. contradiction.
+    * inverts He1.
       assert (value (e_ann (e_ann (e_abs e) (t_arrow A1 B)) A0)). eauto.
       inverts H0. contradiction.
       inverts* H6.
    + inverts* He1. assert (value (e_ann (e_ann (e_abs e) (t_arrow A1 B1)) (t_arrow A2 B2))). eauto.
      inverts H0. contradiction.
-     inverts* H7.
-(*case ste-appr*)
+     inverts H7.
+(*case step-appr*)
   - inverts* He2.
-   + inverts* H. inverts* H0. inverts* H4.
-     assert (value (e_ann (e_lit i5) A0)). eauto.
-     inverts H. contradiction.
-     inverts* H4. assert (value (e_ann (e_ann (e_abs e0) (t_arrow A1 B)) A0)) by auto.
-     inverts H0. contradiction.
+   + inverts* H. inverts* H0. 
+    * inverts* H4. assert (wexpr (e_ann (e_lit i5) A0)) by auto. 
+      contradiction.
+    * inverts H4. assert (wexpr (e_ann (e_bool b) A0)) by auto. contradiction.
+    * inverts H4. assert (wexpr (e_ann (e_str s) A0)) by auto. contradiction.
+    * inverts* H4. assert (wexpr (e_ann (e_ann (e_abs e0) (t_arrow A1 B)) A0)) by auto.
+     contradiction.
      inversion H6.
    + inverts Typ.
      forwards*: IHHe1 H8. rewrite* H0.
      inverts H0. forwards*: IHHe1 H8. rewrite* H0.
-   + inverts H5. inverts H0. inverts H4.
-     inverts He1. inverts H3. contradiction.
-     inverts He1. inverts H3. contradiction.
-     inversion H7.
-     inversion He1.    
+   + inverts H5. inverts H0. inverts H4. 
+    * inverts He1.
+     assert (wexpr (e_ann (e_lit i5) A0)) by auto. contradiction.
+    * inverts He1. assert (wexpr (e_ann (e_bool b) A0)) by auto. contradiction.
+    * inverts He1. assert (wexpr (e_ann (e_str s) A0)) by auto. contradiction.
+    * inverts He1. assert (wexpr (e_ann (e_ann (e_abs e) (t_arrow A3 B)) A0)) by auto.
+      contradiction.
+      inversion H7.
+    * inversion He1.
 (*case step-beta*)
   - inverts* He2.
-   + inverts* H6. assert (value (e_ann (e_ann (e_abs e) (t_arrow A1 B1)) (t_arrow A2 B2))) by auto.
-     inverts H2. contradiction.
+   + inverts* H6. 
+     assert (wexpr (e_ann (e_ann (e_abs e) (t_arrow A1 B1)) (t_arrow A2 B2))) by auto.
+     contradiction.
      inversion H8.
    + inverts H1. inverts H2. inverts H3. 
-     inverts H6. inverts H0. contradiction.
-     inverts H6. inverts H0. contradiction.
-     inversion H8.
-     inversion H6.
+    * inverts H6.
+     assert (wexpr (e_ann (e_lit i5) A0)) by auto. contradiction.
+    * inverts H6. assert (wexpr (e_ann (e_bool b) A0)) by auto. contradiction.
+    * inverts H6. assert (wexpr (e_ann (e_str s) A0)) by auto. contradiction.
+    * inverts H6. assert (wexpr (e_ann (e_ann (e_abs e0) (t_arrow A3 B)) A0)) by auto.
+      contradiction.
+      inversion H8.
+    * inversion H6.
    + inverts H1. inverts H11. auto.
-     inverts H11. auto. 
+     inverts H11. auto.
 (*case step-ann*)
-  - inverts* He2.
-   + inverts Typ. forwards*: IHHe1 H7. rewrite* H0.
-     inverts H0. forwards*: IHHe1 H6. rewrite* H0.
-   + inverts* H3. inverts He1.
-     assert (wexpr (e_ann (e_lit i5) A1)) by auto.
+  - inverts* He2. 
+    inverts Typ. forwards*: IHHe1 H7. rewrite* H0.
+    inverts H0. forwards*: IHHe1 H6. rewrite* H0.
+    inverts H3.
+   + inverts He1. assert (wexpr (e_ann (e_lit i5) A1)) by auto. contradiction.
+   + inverts He1. assert (wexpr (e_ann (e_bool b) A1)) by auto. contradiction.
+   + inverts He1. assert (wexpr (e_ann (e_str s) A1)) by auto. contradiction.
+   + inverts He1. assert (wexpr (e_ann (e_ann (e_abs e) (t_arrow A2 B)) A1)) by auto.
      contradiction.
-     inverts He1.
-     assert (wexpr (e_ann (e_ann (e_abs e)(t_arrow A2 B))A1)) by auto.
-     contradiction.
-     inverts H5.
+     inversion H5.
    + inversion He1.
 (*case step-rm-ann*)
-   - inverts* He2. inverts H. inverts H4.
-    assert (value (e_ann (e_lit i5) A)) by auto.
-    inverts H. contradiction.
-    inverts H4. assert (value (e_ann (e_ann (e_abs e) (t_arrow A1 B0)) A)) by auto.
-    inverts H. contradiction.
-    inversion H6.
+  - inverts* He2. inverts H.
+   + inverts H4. assert (wexpr (e_ann (e_lit i5) A)) by auto. contradiction.
+   + inverts H4. assert (wexpr (e_ann (e_bool b) A)) by auto. contradiction.
+   + inverts H4. assert (wexpr (e_ann (e_str s) A)) by auto. contradiction.
+   + inverts H4. assert (wexpr (e_ann (e_ann (e_abs e) (t_arrow A1 B0)) A)) by auto. contradiction.
+     inversion H6.
 (*case step-lam-ann*)
   - inverts* He2. inversion H4.
-(*case step-typeof*)  
-  - inverts* He2.
+(*case step-typeof*)
+ - inverts* He2.
   + inverts Typ. inverts H0.
     forwards*: IHHe1 H10. rewrite* H0.
-  + inverts* H8. inverts He1.
-    assert (value (e_ann (e_lit i5) D)) by auto.
-    inverts H0. contradiction.
-    inverts He1. assert (value (e_ann (e_ann (e_abs e) (t_arrow A1 B0)) D)) by auto.
-    inverts H1. contradiction.
+  + inverts H8.
+   * inverts He1. assert (wexpr (e_ann (e_lit i5) D)) by auto. contradiction.
+   * inverts He1. assert (wexpr (e_ann (e_bool b) D)) by auto. contradiction.
+   * inverts He1. assert (wexpr (e_ann (e_str s) D)) by auto. contradiction.
+   * inverts He1. assert (wexpr (e_ann (e_ann (e_abs e) (t_arrow A1 B0)) D)) by auto.
+     contradiction.
     inversion H5.
-  + inverts H8. inverts He1.
-    assert (value (e_ann (e_lit i5) D)) by auto.
-    inverts H0. contradiction.
-    inverts He1. assert (value (e_ann (e_ann (e_abs e) (t_arrow A1 B0)) D)) by auto.
-    inverts H1. contradiction.
+  + inverts H8.
+   * inverts He1. assert (wexpr (e_ann (e_lit i5) D)) by auto. contradiction.
+   * inverts He1. assert (wexpr (e_ann (e_bool b) D)) by auto. contradiction.
+   * inverts He1. assert (wexpr (e_ann (e_str s) D)) by auto. contradiction.
+   * inverts He1. assert (wexpr (e_ann (e_ann (e_abs e) (t_arrow A1 B0)) D)) by auto.
+     contradiction.
     inversion H5.
 (*case step-typeofl*)
  - inverts* He2.
-  + inverts H0. inverts H10. assert (value (e_ann (e_lit i5) D)) by auto.
-    inverts H0. contradiction.
-    inverts H10. assert (value (e_ann (e_ann (e_abs e) (t_arrow A1 B0)) D)) by auto.
-    inverts H0. contradiction.
-    inversion H7.
-  + inverts Typ. inverts H3.
-    forwards*: typing_regular. destruct H3.
-    inverts* H1. inverts H12.
-    assert (typing E (e_lit i5) check A); eauto.
-    assert (typing E (e_lit i5) check B); eauto.
-    forwards*: check_both_disj_false H1 H5.
-    inverts H12.
-    unfold DisjSpec in H18. specialize (H18 (t_arrow A1 B0)).
-    forwards*: H18. inversion H1.
-(*case step-typeof*)
- - inverts* He2.
-  + inverts H1. inverts H10. assert (value (e_ann (e_lit i5) D)) by auto.
-    inverts H1. contradiction.
-    inverts H10. assert (value (e_ann (e_ann (e_abs e) (t_arrow A1 B0)) D)) by auto.
-    inverts H1. contradiction.
-    inversion H7.
-  + inverts Typ. inverts H3.
-    forwards*: typing_regular. destruct H3.
-    inverts* H1. inverts H12.
-    unfold DisjSpec in H18. specialize (H18 t_int).
-    forwards*: H18. inversion H1.
-    inverts H12.
-    unfold DisjSpec in H18. specialize (H18 (t_arrow A1 B0)).
-    forwards*: H18. inversion H1.
-Qed.
-
-Lemma determinism : forall E e e1 e2 A, typing E e check A -> 
-e --> e1 -> e --> e2 -> e1 = e2.
-Proof.
-  introv Typ He1. gen e2 A.
-  induction He1; introv Typ He2.
-(*case step-int*)
-  - inverts* He2.
-(*case step-appl*)
-  - inverts* He2.
-   + inverts Typ. inverts H0. eapply typ_sub with (A:=(t_arrow A0 B)) in H7; eauto.
-     forwards*: IHHe1. rewrite* H0.
-   + inverts* H2. inverts* H0. 
-    * inverts* He1. unfold not in H2. 
-      assert (value (e_ann (e_lit i5) A0)). eauto.
-      inverts H0.
-      apply H2 in H1. inversion H1.
-    * inverts* He1. unfold not in H3.
-      assert (value (e_ann (e_ann (e_abs e) (t_arrow A1 B)) A0)). eauto.
-      inverts H0.
-      apply H3 in H2. inversion H2.
-      inverts* H6.
-   + inverts* He1. assert (value (e_ann (e_ann (e_abs e) (t_arrow A1 B1)) (t_arrow A2 B2))). eauto.
-     inverts H0.
+  + inverts H1. 
+   * inverts H10. assert (wexpr (e_ann (e_lit i5) D)) by auto. contradiction.
+   * inverts H10. assert (wexpr (e_ann (e_bool b) D)) by auto. contradiction.
+   * inverts H10. assert (wexpr (e_ann (e_str s) D)) by auto. contradiction.
+   * inverts H10. assert (wexpr (e_ann (e_ann (e_abs e) (t_arrow A1 B0)) D)) by auto.
      contradiction.
-     inverts H7.
-(*case step-appr*)
-  - inverts* He2.
-   + inverts* H. inverts* H0. inverts* H4.
-     assert (value (e_ann (e_lit i5) A0)). eauto.
-     inverts H. contradiction.
-     inverts* H4. assert (value (e_ann (e_ann (e_abs e0) (t_arrow A1 B)) A0)) by auto.
-     inverts H0. contradiction.
-     inversion H6.
-   + inverts Typ. inverts H0. forwards*: IHHe1 H8. rewrite* H0.
-   + inverts H5. inverts H0. inverts H4.
-     inverts He1. inverts H3. contradiction.
-     inverts He1. inverts H3. contradiction.
-     inversion H7.
-     inversion He1.     
-(*case step-beta*)
-  - inverts* He2.
-   + inverts* H6. assert (value (e_ann (e_ann (e_abs e) (t_arrow A1 B1)) (t_arrow A2 B2))) by auto.
-     inverts H2. contradiction.
-     inverts H8.
-   + inverts H1. inverts H2. inverts H3.
-     inverts H6. inverts H0. contradiction.
-     inverts H6. inverts H0. contradiction.
-     inversion H8.
-     inversion H6.
-   + inverts H1. inverts H11. auto.
-     inverts H11. auto. 
-(*case step-ann*)
-  - inverts* He2.
-   + inverts Typ. inverts H0.
-     forwards*: IHHe1. rewrite* H0.
-   + inverts* H3. inverts* He1.
-     assert (value (e_ann (e_lit i5) A1)) by auto.
-     inverts H0. contradiction.
-     inverts He1. assert (value (e_ann (e_ann (e_abs e) (t_arrow A2 B)) A1)) by auto.
-     inverts H1. contradiction.
-     inversion H5.
-   + inverts* He1.
-(*case step-rm-ann*) 
-  - inverts* He2. inverts H. inverts H4.
-    assert (value (e_ann (e_lit i5) A)) by auto.
-    inverts H. contradiction.
-    inverts H4. assert (value (e_ann (e_ann (e_abs e) (t_arrow A1 B0)) A)) by auto.
-    inverts H. contradiction.
-    inversion H6.
-(*case step-lam-ann*)
-  - inverts* He2. inversion H4.
-(*case step-typeof*)
-  - inverts* He2.
-  + inverts Typ. inverts H0.
-    forwards*: IHHe1 H5. rewrite* H0.
-  + inverts* H8. inverts He1.
-    assert (value (e_ann (e_lit i5) D)) by auto.
-    inverts H0. contradiction.
-    inverts He1. assert (value (e_ann (e_ann (e_abs e) (t_arrow A1 B0)) D)) by auto.
-    inverts H1. contradiction.
-    inversion H5.
-  + inverts H8. inverts He1.
-    assert (value (e_ann (e_lit i5) D)) by auto.
-    inverts H0. contradiction.
-    inverts He1. assert (value (e_ann (e_ann (e_abs e) (t_arrow A1 B0)) D)) by auto.
-    inverts H1. contradiction.
-    inversion H5.
-(*case setp-typeofl*)
- - inverts* He2.
-  + inverts H0. inverts H10. assert (value (e_ann (e_lit i5) D)) by auto.
-    inverts H0. contradiction.
-    inverts H10. assert (value (e_ann (e_ann (e_abs e) (t_arrow A1 B0)) D)) by auto.
-    inverts H0. contradiction.
     inversion H7.
   + inverts Typ. inverts H3.
     forwards*: typing_regular. destruct H3.
-    inverts* H1. inverts H12.
-    assert (typing E (e_lit i5) check A); eauto.
-    assert (typing E (e_lit i5) check B); eauto.
-    forwards*: check_both_disj_false H1 H5.
-    inverts H12.
-    unfold DisjSpec in H17. specialize (H17 (t_arrow A1 B0)).
-    forwards*: H17. inversion H1.
-(*case typeofr*)
- - inverts* He2.
-  + inverts H1. inverts H10. assert (value (e_ann (e_lit i5) D)) by auto.
-    inverts H1. contradiction.
-    inverts H10. assert (value (e_ann (e_ann (e_abs e) (t_arrow A1 B0)) D)) by auto.
-    inverts H1. contradiction.
-    inversion H7.
-  + inverts Typ. inverts H3.
-    forwards*: typing_regular. destruct H3.
-    inverts* H1. inverts H12.
-    unfold DisjSpec in H17. specialize (H17 t_int).
-    forwards*: H17. inversion H1.
-    inverts H12.
-    unfold DisjSpec in H17. specialize (H17 (t_arrow A1 B0)).
-    forwards*: H17. inversion H1.
+    inverts* H1. 
+   * inverts H12.
+     unfold DisjSpec in H18. specialize (H18 t_int).
+     forwards*: H18.
+     unfold not in H1.
+     forwards*: H1.
+    * inverts H12.
+      unfold DisjSpec in H18. specialize (H18 t_bool).
+      forwards*: H18.
+      unfold not in H1.
+      forwards*: H1.
+    * inverts H12.
+      unfold DisjSpec in H18. specialize (H18 t_str).
+      forwards*: H18.
+      unfold not in H1.
+      forwards*: H1.
+   * inverts H12.
+     unfold DisjSpec in H18. specialize (H18 (t_arrow A1 B0)).
+     forwards*: H18.
+     unfold not in H1.
+     forwards*: H1.
+(*case step-typeofr*) 
+- inverts* He2.
+     + inverts H1. 
+      * inverts H10. assert (wexpr (e_ann (e_lit i5) D)) by auto. contradiction.
+      * inverts H10. assert (wexpr (e_ann (e_bool b) D)) by auto. contradiction.
+      * inverts H10. assert (wexpr (e_ann (e_str s) D)) by auto. contradiction.
+      * inverts H10. assert (wexpr (e_ann (e_ann (e_abs e) (t_arrow A1 B0)) D)) by auto.
+        contradiction.
+       inversion H7.
+     + inverts Typ. inverts H3.
+       forwards*: typing_regular. destruct H3.
+       inverts* H1. 
+      * inverts H12.
+        unfold DisjSpec in H18. specialize (H18 t_int).
+        forwards*: H18.
+        unfold not in H1.
+        forwards*: H1.
+       * inverts H12.
+         unfold DisjSpec in H18. specialize (H18 t_bool).
+         forwards*: H18.
+         unfold not in H1.
+         forwards*: H1.
+       * inverts H12.
+         unfold DisjSpec in H18. specialize (H18 t_str).
+         forwards*: H18.
+         unfold not in H1.
+         forwards*: H1.
+      * inverts H12.
+        unfold DisjSpec in H18. specialize (H18 (t_arrow A1 B0)).
+        forwards*: H18.
+        unfold not in H1.
+        forwards*: H1.
 Qed.
